@prefix : <http://purl.org/ascaris/docta/> .
@prefix dcterms: <http://purl.org/dc/terms/> .
@prefix owl: <http://www.w3.org/2002/07/owl#> .
@prefix rdfs: <http://www.w3.org/2000/01/rdf-schema#> .
@prefix skos: <http://www.w3.org/2004/02/skos/core#> .
@prefix vann: <http://purl.org/vocab/vann/> .
@prefix xsd: <http://www.w3.org/2001/XMLSchema#> .

:document a skos:Concept ;
    rdfs:label "document"@en ;
    skos:prefLabel "Document"@en ;
    skos:definition "A written or printed piece of information that serves as a record, proof, or evidence of something."@en ;
    skos:topConceptOf :document-type-taxonomy ;
    skos:inScheme :document-type-taxonomy ;
    dcterms:creator <https://orcid.org/0000-0002-0799-1527> ;
    dcterms:created "2023-08-31"^^xsd:date .

:book a skos:Concept ;
    rdfs:label "book"@en ;
    skos:prefLabel "Book"@en ;
    skos:definition "A physical or digital document that contains written, printed, or illustrated content organized into pages, chapters, or sections."@en ;
    skos:broader :document ;
    skos:inScheme :document-type-taxonomy ;
    dcterms:creator <https://orcid.org/0000-0002-0799-1527> ;
    dcterms:created "2023-08-31"^^xsd:date .

:letter a skos:Concept ;
    rdfs:label "letter"@en ;
    skos:prefLabel "Letter"@en ;
    skos:definition "A physical document that contains written content, typically sent from one individual or entity to another."@en ;
    skos:broader :document ;
    skos:inScheme :document-type-taxonomy ;
    dcterms:creator <https://orcid.org/0000-0002-0799-1527> ;
    dcterms:created "2023-08-31"^^xsd:date .

:document-type-taxonomy a skos:ConceptScheme ;
    rdfs:label "Document Type Taxonomy"@en ;
    dcterms:title "Document Type Taxonomy (DocTa)"@en ;
    dcterms:identifier "todo" ;
    dcterms:rights <https://creativecommons.org/licenses/by/4.0/> ;
    dcterms:created "2023-08-31"^^xsd:date ;
    dcterms:creator <https://orcid.org/0000-0002-0799-1527> ;
    dcterms:bibliographicCitation "todo"@en ;
    vann:preferredNamespacePrefix "docta";
    owl:versionInfo "0.1.0" ;
    skos:definition "A SKOS controlled taxonomy of document types."@en ;
    skos:scopeNote "https://www.purl.org/ascaris/docta/ is the namespace of the taxonomy. Its preferred prefix is `docta`. In order to understand the meaning of any concept, please refer to its respective documentation properties, such as `skos:prefLabel`."@en .